## **Lucas' Theorem for Prime Powers**

KENNETH S. DAVIS AND WILLIAM A. WEBB

Lucas' theorem on binomial coefficients states that  $\binom{A}{B} = \binom{a_1}{b_1} \cdots \binom{a_0}{b_1} \pmod{p}$  where p is a prime and  $A = a_r p^r + \cdots + a_1 p + a_0$ ,  $B = b_r p^r + \cdots + b_1 p + b_0$  are the p-adic expansions of A and B. If  $s \ge 2$ , it is shown that a similar formula holds modulo  $p^s$  where the product involves a slightly modified binomial coefficient evaluated on blocks of s digits.

## Introduction

One of the most beautiful results concerning binomial coefficients is Lucas' Theorem [1,2]. If  $0 \le B \le A$  are integers and p is a prime, write A and B in p-adic notation  $A = a_r p^r + \cdots + a_1 p + a_0$ ,  $B = b_r p^r + \cdots + b_1 p + b_0$ , where  $0 \le a_i$ ,  $b_i < p$  and  $a_r \ne 0$ . Then

$$\binom{A}{B} \equiv \binom{a_r}{b_r} \binom{a_{r-1}}{b_{r-1}} \cdots \binom{a_1}{b_1} \binom{a_0}{b_0} \pmod{p}.$$
 (1)

If  $A - B = c_r p^r + \cdots + c_1 p + c_0$  and  $p^t \mid \binom{A}{B}$  then Kazandzidis [3] proved that

$$\binom{A}{B} \equiv (-p^t) \prod_{i=0}^r \frac{a_i!}{b!! c_i!} \pmod{p^{t+1}}.$$

This result is applicable for only one power of p for each  $\binom{A}{B}$ , and in particular does not apply for  $t \ge 1$  if  $\binom{A}{B}$ ,  $p \ge 1$ . Singmaster [5] also obtained similar results.

For integers A and B as above, define the string  $A_{ij} = a_i a_{i-1} \cdots a_j$  for  $0 \le j \le i \le r$ , with  $B_{ij}$  defined similarly. Corresponding to a string  $A_{ij}$  is the integer  $\mathcal{A}_{ij} = a_i p^{i-j} + \cdots + a_{j+1}p + a_j$ . Let  $\le$  be the lexical order on strings, so that  $A_{ij} \le B_{ij}$  iff  $\mathcal{A}_{ij} \le \mathcal{B}_{ij}$ , with  $O_i$  denoting the string of i+1 zeros.

We also define a modified binomial coefficient on such strings as follows. In the following assume j is fixed and write  $A_i = A_{ij}$ , etc. Also  $p^s$  is a fixed power of p.

If  $B_i \leq A_i$  then  $\langle A_i \rangle = \langle A_i \rangle = \langle A_i \rangle$ .

If  $A_0 < B_0$  then  $\langle A_0 \rangle = p$ , and recursively if  $A_i < B_i$ ,  $i \ge 1$ , then  $\langle A_i \rangle = p \langle A_{i-1} \rangle$ .

In general  $\langle A_i \rangle = p'\alpha$ , where  $t \ge 0$  and  $p \mid \alpha$ .

Formally,  $\langle A_i \rangle^{-1} = p^{-t} \alpha^{-1}$ , where  $\alpha^{-1}$  is such that  $\alpha \alpha^{-1} \equiv 1 \pmod{p^s}$  and  $0 < \alpha^{-1} < p^s$ . The following properties are clear:

- $(1) \langle {}^{A_i}_{B_i} \rangle \langle {}^{A_i}_{B_i} \rangle^{-1} \equiv 1 \pmod{p^s}.$
- (2) If  $A_k \ge B_k$  and  $A_{k+l} < B_{k+l}$  for  $1 \le l \le i-k$  then  $\binom{A_i}{B_i} = p^{i-k} \binom{A_k}{B_k}$ .
- (3) Suppose  $p^t \parallel \langle A_i \rangle$ . If  $A_i \ge B_i$  then it is well known that t is the number of borrows necessary in the subtraction  $\mathcal{A}_i \mathcal{B}_i$ . [4] If  $A_i < B_i$  then t is the number of borrows in the subtraction  $(p^{i+1} + \mathcal{A}_i) \mathcal{B}_i$ . Thus if  $\langle A_{i+1} \rangle \langle A_i \rangle^{-1} = p'\alpha$ , where  $p \mid \alpha$ , then  $t \ge 0$ .

Our goal is to prove the following generalization of Lucas' Theorem which completely determines the value of any binomial coefficient modulo any prime power.

THEOREM 1. For any integers  $0 \le B \le A$  and any prime power  $p^s$ ,  $2 \le s \le r + 1$ ,

1. For any unegers 
$$0 \le B \le A$$
 and any prime power  $p$ ,  $2 \le s \le r + 1$ ,
$$\begin{pmatrix} A \\ B \end{pmatrix} \equiv \begin{pmatrix} a_{s-1} \cdots a_0 \\ b_{s-1} \cdots b_0 \end{pmatrix} \prod_{j=1}^{r-s+1} \begin{pmatrix} a_{j+s-1} \cdots a_j \\ b_{j+s-1} \cdots b_j \end{pmatrix} \begin{pmatrix} a_{j+s-2} \cdots a_j \\ b_{j+s-2} \cdots b_j \end{pmatrix}^{-1}$$

$$\equiv \begin{pmatrix} A_{s-1} \\ B_{s-1} \end{pmatrix} \prod_{j=1}^{r-s+1} \begin{pmatrix} A_{j+s-1,j} \\ B_{j+s-1,j} \end{pmatrix} \begin{pmatrix} A_{j+s-2,j} \\ B_{j+s-2} \end{pmatrix}^{-1}$$
(mod  $p^s$ ).

The modified binomial coefficients are needed only in evaluating  $\binom{A_j}{B_j}$ , where  $B_j > A_j$ , so we have as an immediate corollary.

COROLLARY. If  $b_i \leq a_i$  for  $0 \leq i \leq r$  then

$$\binom{A}{B} \equiv \binom{\mathcal{A}_{s-1}}{\mathcal{B}_{s-1}} \prod_{j=1}^{r-s+1} \binom{\mathcal{A}_{j+s-1,j}}{\mathcal{B}_{j+s-1,j}} \binom{\mathcal{A}_{j+s-2,j}}{\mathcal{B}_{j+s-2,j}}^{-1} \pmod{p^s}.$$

The following example illustrates how this theorem can be used in a specific case. Note that we can always reduce the calculation to ordinary binomial coefficients.

Let p = 7 and s = 3, and suppose that the base 7 representations of A and B are A = 2413605 and B = 1261632.

## PROOF OF THEOREM 1

The following lemma will be useful.

LEMMA:

$$\binom{pA}{pB} = \binom{A}{B} \prod_{i=1}^{p-1} \prod_{k=1}^{B} \frac{p(k+A-B)-j}{pk-j}$$

for integer  $0 \le B \le A$ .

Proof:

and the result follows by cancelling  $p^B$  in the first factor.

Our proof of Theorem 1 uses induction on A. It is trivial for A < p. From now on let  $A_i = A_{io}$  etc. Let  $\prod \langle A_r, B_r \rangle = \prod \langle A, B \rangle$  denote a product of the type on the right side of (2), and

$$\prod^* \langle A, B \rangle = \prod \langle A, B \rangle {A_{s-1} \choose B_{s-1}}^{-1}.$$

The result is also clear for r = s - 1 since  $\binom{A}{B} = \binom{A_r}{B_r}$ , so we may assume  $r \ge s$ .

Assume that (2) holds for all integers A' less than A and all  $B \le A'$  and suppose that  $A = a_r p' + \cdots + a_0$ ,  $a_r \ne 0$ .

We consider several cases, depending on the values of  $a_0$  and  $b_0$ .

Case 1:  $a_0 = 0$  and  $b_0 = 0$ . Let  $\alpha_k = a_k p^{k-1} + \dots + a_1$  and  $\beta_k = b_k p^{k-1} + \dots + b_1$ , so  $A = \mathcal{A}_{r,0} = p\alpha_r$  and  $B = \mathcal{B}_{r,0} = p\beta_r$ . Hence,

$$\binom{A}{B} = \binom{p\alpha_r}{p\beta_r} = \binom{\alpha_r}{\beta_r} \prod_{j=1}^{p-1} \prod_{k=1}^{\beta_r} \frac{p(k+\alpha_r-\beta_r)-j}{pk-j}$$
 (3)

by the lemma.

Since  $0 \le \beta_r \le \alpha_r < A$ , we may apply the induction hypothesis to  $\binom{\alpha_r}{\beta_r}$ . We also note that formally, the expressions for  $\prod \langle A, B \rangle$  and  $\prod \langle \alpha_r, \beta_r \rangle$  are identical except for two factors. Hence,

$$\prod \langle A_r, B_r \rangle = \prod \langle \alpha_r, \beta_r \rangle \left\langle \begin{matrix} a_{s-1} \cdots a_1 0 \\ b_{s-1} \cdots b_1 0 \end{matrix} \right\rangle \left\langle \begin{matrix} a_{s-1} \cdots a_1 \\ b_{s-1} \cdots b_1 \end{matrix} \right\rangle^{-1} \\
= \left(\begin{matrix} \alpha_r \\ \beta_r \end{matrix} \right) \left\langle \begin{matrix} A_{s-1} \\ B_{s-1} \end{matrix} \right\rangle \left\langle \begin{matrix} A_{s-1,1} \\ B_{s-1,1} \end{matrix} \right\rangle^{-1}.$$
(4)

If  $p^s \mid {\alpha \choose \beta'}$  then both sides of (2) are zero and case 1 is settled. Otherwise, let  $p^{\lambda} \parallel {\alpha \choose \beta'}$  where  $\lambda < s$ . Then comparing (3) and (4), equation (2) holds iff

$$\prod_{j=1}^{p-1} \prod_{k=1}^{\beta_r} \frac{p(k+\alpha_r-\beta_r)-j}{pk-j} = \left\langle \frac{A_{s-1}}{B_{s-1}} \right\rangle \left\langle \frac{A_{s-1,1}}{B_{s-1,1}} \right\rangle^{-1} (\text{mod } p^{s-\lambda}).$$
 (5)

By earlier remarks,

$$\left\langle \begin{matrix} A_{s-1} \\ B_{s-1} \end{matrix} \right\rangle = p^t \left\langle \begin{matrix} A_u \\ B_u \end{matrix} \right\rangle,$$

where  $A_u \ge B_u$  for some  $u \ge 0$ ,  $0 \le t < s$ . If u = 0,

$$\left\langle \begin{matrix} A_{s-1} \\ B_{s-1} \end{matrix} \right\rangle = p^{s-1} = \left\langle \begin{matrix} A_{s-1,1} \\ B_{s-1,1} \end{matrix} \right\rangle$$

and the right hand side of (5) is 1. For u > 0, we also have

$$\left\langle \begin{matrix} A_{s-1,1} \\ B_{s-1,1} \end{matrix} \right\rangle = p^t \left\langle \begin{matrix} A_{u,1} \\ B_{u,1} \end{matrix} \right\rangle$$

and so the right side of (5) becomes

$$p' \left\langle \begin{matrix} A_t \\ B_u \end{matrix} \right\rangle p^{-t} \left\langle \begin{matrix} A_{u,1} \\ B_{u,1} \end{matrix} \right\rangle^{-1} \equiv \left( \begin{matrix} \mathcal{A}_u \\ \mathcal{B}_u \end{matrix} \right) \left\langle \begin{matrix} \alpha_u \\ \beta_u \end{matrix} \right\rangle^{-1}$$

$$= \left( \begin{matrix} p \alpha_u \\ p \beta_u \end{matrix} \right) \left\langle \begin{matrix} \alpha_u \\ \beta_u \end{matrix} \right\rangle^{-1} \equiv \left( \begin{matrix} \alpha_u \\ \beta_u \end{matrix} \right) \prod_{j=1}^{p-1} \prod_{k=1}^{\beta_u} \frac{p(k + \alpha_u - \beta_u) - j}{pk - j} \left\langle \begin{matrix} \alpha_u \\ \beta_u \end{matrix} \right\rangle^{-1}$$

$$= \prod_{j=1}^{p-1} \prod_{k=1}^{\beta_u} \frac{p(k + \alpha_u - \beta_u) - j}{pk - j} \pmod{p^s}.$$

Thus it now suffices to show

$$\prod_{i=1}^{p-1} \prod_{k=1}^{\beta_r} \frac{p(k+\alpha_r-\beta_r)-j}{pk-j} \equiv \prod_{i=1}^{p-1} \prod_{k=1}^{\beta_u} \frac{p(k+\alpha_r-\beta_r)-j}{pk-j} \pmod{p^{s-\lambda}}.$$
 (6)

Also, since  $t \le \lambda$  it suffices to prove (6) modulo  $p^{s-t} = p^{u+1}$ . Finally, since  $p(\alpha_r - \beta_r) \equiv p(\alpha_u - \beta_u) \pmod{p^{u+1}}$ , it suffices to show

$$\prod_{j=1}^{p-1} \prod_{k=\beta_{u}+1}^{\beta_{r}} \frac{p(k+\alpha_{r}-\beta_{r})-j}{pk-j} \equiv 1 \pmod{p^{s-\lambda}}.$$
 (7)

We observe that px-j runs over a reduced residue system modulo  $p^{u+1}$  as  $1 \le j \le p-1$  and x runs over any  $p^u$  consecutive integers. In (7), k runs over  $\beta_r - \beta_u = b_r p^r + \cdots + b_{u+1} p^u$  consecutive integers. This in (7), both  $p(k + \alpha_r - \beta_r) - j$  and pk-j runs over a reduced residue system modulo  $p^{u+1}$ , exactly  $b_r p^{r-u} + \cdots + b_{u+1}$  times, which proves (7).

Case 2:  $a_0 \neq 0$  and  $b_0 \neq 0$ . The result is trivial if A = B. If  $A \geq B + 1$  then (3) follows immediately from applying the induction hypothesis to  $\binom{A-1}{B}$  and  $\binom{A-1}{B-1}$  and noting that

$$\left\langle a_{s-1} \cdot \cdot \cdot a_1 a_0 - 1 \right\rangle + \left\langle a_{s-1} \cdot \cdot \cdot a_1 a_0 - 1 \right\rangle = \left\langle a_{s-1} \cdot \cdot \cdot a_1 a_0 \right\rangle.$$

Case 3:  $a_0 \ne 0$  and  $b_0 = 0$ . We note that  $p \mid B + 1$  and  $p \mid A - B$  and, furthermore,

$$\binom{A}{B} = \binom{A}{B+1} \frac{B+1}{A-B}.$$

By Case 2, equation (3) holds for  $\binom{A}{B+1}$  and so it suffices to show that

$$p^{s} \mid \prod^{*} {A_{s-1} \choose B_{s-1}} - \prod^{*} {A_{s-1} \choose B_{s-1} + 1} \frac{B+1}{A-B}$$

where  $\Pi^* = \Pi^* \langle A, B \rangle = \Pi^* \langle A, B+1 \rangle$ . Since  $A = \mathcal{A}_{s-1}$  and  $B = \mathcal{B}_{s-1} \pmod{p^s}$  we must show that

$$p^{s} \mid \prod^{*} \left( \left\langle \begin{matrix} A_{s-1} \\ B_{s-1} \end{matrix} \right\rangle (\mathcal{A}_{s-1} - \mathcal{B}_{s-1}) - \left\langle \begin{matrix} A_{s-1} \\ B_{s-1} + 1 \end{matrix} \right\rangle (\mathcal{B}_{s-1} + 1) \right).$$

Now,

$$\left\langle \begin{matrix} A_{s-1} \\ B_{s-1} \end{matrix} \right\rangle = p^t \left\langle \begin{matrix} A_u \\ B_u \end{matrix} \right\rangle,$$

where  $A_u > B_u$  for some u = s - t - 1 > 0, and also

$$\left\langle \begin{matrix} A_{s-1} \\ B_{s-1} + 1 \end{matrix} \right\rangle = p^{t} \left\langle \begin{matrix} A_{u} \\ B_{u} + 1 \end{matrix} \right\rangle,$$

where  $A_u \ge B_u + 1$ . By earlier remarks  $\Pi^*$  is divisible by a non-negative power of p and so it suffices to show that

$$p^{s-t} \left| \left( \left\langle \begin{matrix} A_u \\ B_u \end{matrix} \right) (\mathcal{A}_{s-1} - \mathcal{B}_{s-1}) - \left\langle \begin{matrix} A_u \\ B_u + 1 \end{matrix} \right) (\mathcal{B}_{s-1} + 1) \right|. \tag{8}$$

But  $p^{s-t} = p^{u+1}$  and  $\mathcal{A}_{s-1} \equiv \mathcal{A}_u$ ,  $\mathcal{B}_{s-1} \equiv \mathcal{B}_u$  modulo  $p^{u+1}$ , and

so equation (8) holds.

Case 4:  $a_0 = 0$  and  $b_0 \neq 0$ . This is similar to Case 3. By Case 1, the theorem holds for  $\binom{A}{B}$ , where  $b_0 = 0$  and  $a_0 = 0$ . For A fixed,  $a_0 = 0$ , assume true for  $\binom{A}{B}$ , where  $0 \leq b_0 \leq p-2$ , and note that

$$\binom{A}{B+1} = \binom{A}{B} \frac{A-B}{B+1}$$

where  $p \mid A - B$  and  $p \mid B + 1$ . As before, it suffices to show that

$$p^{s} \left| \prod^{*} \left( \left\langle \frac{A_{s-1}}{B_{s-1} + 1} \right\rangle (\mathcal{B}_{s-1} + 1) - \left\langle \frac{A_{s-1}}{B_{s-1}} \right\rangle (\mathcal{A}_{s-1} - \mathcal{B}_{s-1}) \right).$$
 (9)

It may happen that

$$\left\langle \begin{matrix} A_{s-1} \\ B_{s-1} + 1 \end{matrix} \right\rangle = p^s = \left\langle \begin{matrix} A_{s-1} \\ B_{s-1} \end{matrix} \right\rangle,$$

in which case (9) is immediate. Otherwise,

$$\binom{A_{s-1}}{B_{s-1}+1}=p^{t}\binom{A_{u}}{B_{u}+1},$$

where  $A_u \ge B_u + 1$  and the rest is the same as Case 3.

## REFERENCES

- 1. L. E. Dickson, History of the theory of numbers, Vol. 1, Chelsea, New York, 1952.
- 2. N. J. Fine, Binomial coefficients modulo a prime, Am. Math. Monthly, 54 (1947), 589-592.
- 3. G. S. Kazandzidis, Congruences on binomial coefficients, Bull. Soc. Math. Grèce (NS), 9 (1968), 1-12.
- 4. D. Singmaster, Divisibility of binomial and multinomial coefficients by primes and prime powers, From a collection of manuscripts related to the Fibonacci Sequence.
- D. Singmaster, Notes on binomial coefficients I—a generalization of Lucas' congruence, J. Lond. Math. Soc. (2), 8 (1974), 545-548.

Received 16 May 1989 and accepted 15 January 1990

KENNETH S. DAVIS
Albion College,
Department of Mathematics,
Albion, Michigan 49224, U.S.A.

WILLIAM A. WEBB Washington State University, Department of Pure and Applied Mathematics, Pullman, Washington 99164-2930, U.S.A.